upd

Spec.Claim.fst
@@ -1,6 +1,10 @@
 module Spec.Claim
 
 open FStar.Seq
+open SkipList2.Statement
+open SkipList2.Insertion2
+open SkipList2.Properties
+open SkipList2.Search
 
 let bytes =  seq FStar.UInt8.t
 
@@ -13,12 +17,13 @@ type indentifier =
 assume val hash: list 'a -> bytes
 
 type metadata = 
-|InitMetadata: screen_name: option string ->
-				real_name: option string -> 
-				identifiers: list indentifier -> 
-				keys: list keyEnt -> 
-				hashMetadata: bytes ->
-				metadata
+	|InitMetadata: screen_name: option string ->
+		real_name: option string -> 
+		identifiers: list indentifier ->
+		keys: list keyEnt -> 
+		hashMetadata: bytes ->
+		metadata
+	|NullMetadata : metadata				
 
 
 
@@ -28,11 +33,114 @@ assume val verify : signature: bytes -> data: bytes -> Tot bool
 assume val toBytes: input : 'a -> bytes
 assume val concat: bytes-> bytes -> bytes
 
+assume val signVerif: input: bytes -> 
+	Lemma 
+	(ensures (verify (sign input) input == true ))
+
 (* Authenticity of information *)
+
+type time = nat
+
 type claim = 
-	|InitClaim: test: list int -> signature : bytes{verify signature (toBytes test) } -> claim (* test purposes*)
-	|KeyBindingClaim: meta: metadata -> key: bytes -> signature : bytes {verify signature (concat (toBytes meta) (toBytes key))}  -> claim
-	|ClaimChainState: id: bytes -> state: bytes-> signature : bytes{verify signature (concat id state)} -> claim
-	|Revocation: id: bytes -> signature : bytes{verify signature id}-> claim
+	|InitClaim: 
+		timeStamp: (k : time{k = 0}) ->  
+		test: list int -> 
+		signature : bytes{verify signature (toBytes test) } -> claim (* test purposes*)
+	|KeyBindingClaim: 
+		timeStamp : (k : time { k> 0}) -> 
+		meta: metadata -> 
+		key: bytes -> 
+		signature : bytes {verify signature (concat (toBytes meta) (toBytes key))}  -> claim
+	|ClaimChainState: 
+		timeStamp: (k : time { k> 0}) -> 
+		id: bytes -> 
+		state: bytes-> 
+		signature : bytes{verify signature (concat id state)} -> claim
+	|Revocation: 
+		timeStamp : (k : time { k> 0}) -> 
+		id: bytes -> 
+		signature : bytes{verify signature id}-> claim
+
+val getTimeStamp: cl: claim -> time
+let getTimeStamp cl = 
+	match cl with
+	| InitClaim timeStamp _ _ -> timeStamp
+	| KeyBindingClaim timeStamp _ _ _ -> timeStamp
+	| ClaimChainState timeStamp _ _ _  -> timeStamp
+	| Revocation timeStamp _ _ -> timeStamp
+
+val func_ord_claim: claim1: claim -> claim2: claim -> Tot(r: bool)
+let func_ord_claim claim1 claim2 = 
+	if claim1 = claim2 then true else
+	getTimeStamp claim1 < getTimeStamp claim2
 
 
+type cmp (a:eqtype) =  f:(a -> a -> Tot bool){total_order a f}
+type cmpClaim = f: (claim -> claim -> Tot bool) {total_order claim f}
+
+val getClaimMax: unit -> Tot claim
+let getClaimMax () = 
+	let l = [0] in 
+	let data = toBytes l  in 
+	let signature =  sign data in 
+	signVerif data; assert(verify (sign data) data == true);
+	InitClaim 0 l signature  
+
+type claimCh (f: cmpClaim ) = skipList claim f
+
+val createEmptyClaimChaim : #f: cmpClaim -> size: nat {size > 0} -> claimCh f
+
+let createEmptyClaimChaim #f size= 
+	SkipList2.Statement.create #claim #f (getClaimMax()) size
+
+val addClaim:  #f: cmpClaim ->  cl: claim -> max_level: nat ->chain : claimCh f{SkipList2.Statement.length chain > 0} -> claimCh f
+let addClaim #f cl max_level chain = 
+	match cl with 
+		|InitClaim _ _ _ -> chain
+		| _ -> 
+			assert(getTimeStamp cl > 0);
+			SkipList2.Properties.lemma_last_element_biggest #claim #f chain cl;
+			assert(f cl (last_element_values #claim #f chain));
+			if (Seq.mem cl (SkipList2.Statement.getValues chain) = true) 
+				then chain 
+			else 
+			(
+				assert (Seq.mem cl (SkipList2.Statement.getValues chain) = false);
+				SkipList2.Insertion2.addition #claim #f cl chain max_level				
+			)
+				
+
+
+val getFirstElement: #f: cmpClaim -> chain: claimCh f{SkipList2.Statement.length chain > 0} -> Tot claim
+let getFirstElement #f chain = 
+	SkipList2.Statement.hd #claim #f chain
+
+
+val getLastElement : #f: cmpClaim -> chain : claimCh f{SkipList2.Statement.length chain > 0} -> Tot claim
+let getLastElement #f chain = 
+	last_element_values #claim #f chain
+
+(*val nextElement: #a: eqtype -> #f: cmp a -> sl: skipList a f {Sl.length sl > 1}-> element: a -> Tot(option (a))*)
+val getNextElement : #f : cmpClaim -> chain : claimCh f {SkipList2.Statement.length chain > 1} -> cl: claim -> Tot (option (claim))
+let getNextElement #f chain cl = 
+	SkipList2.Search.nextElement #claim #f chain cl 
+
+val getPreviousElement: #f: cmpClaim -> chain : claimCh f {SkipList2.Statement.length chain > 1} -> cl: claim -> Tot(option (claim))
+let getPreviousElement #f chain cl = 
+	SkipList2.Search.prevElement #claim #f chain cl
+
+(*)
+let func_ord_claim_lemma () : Lemma (total_order claim func_ord_claim) = ()
+
+let comp = func_ord_claim
+
+val func_ord_claim4 : unit -> f:(claim -> claim -> Tot bool)
+let func_ord_claim4 () = comp
+
+type total_order (a:eqtype) (f: (a -> a -> Tot bool)) =
+    (forall a. f a a)                                           (* reflexivity   *)
+    /\ (forall a1 a2. (f a1 a2 /\ a1<>a2)  <==> not (f a2 a1))  (* anti-symmetry *)
+    /\ (forall a1 a2 a3. f a1 a2 /\ f a2 a3 ==> f a1 a3)        (* transitivity  *)
+type tot_ord (a:eqtype) = f:(a -> a -> Tot bool){total_order a f}
+(*)
+let func_ord_claim4 cmp claim = func_ord_claim
