Spec.ClaimChain.fst
@@ -2,30 +2,175 @@ module Spec.ClaimChain
 
 open FStar.Seq
 open Spec.Claim
+open SkipList2.Statement
+
+open HashFunction
+open FStar.Constructive
 
 let bytes =  seq FStar.UInt8.t
+(*)
 
-type claimChain = 
-|InitChaimChain : 
-			id: bytes -> 
+type path = list bool
+
+val get_elt:  #h:hash -> path:path -> tree:merkleTree (List.length path) h -> f: cmpClaim -> Tot data f
+             (decreases path)
+let rec get_elt #h path tree =
+  match path with
+    | [] -> MLeaf?.element tree
+    | bit::path' ->
+      if bit then
+  get_elt #(MNode?.h1 tree) path' (MNode?.lnode tree)
+      else
+  get_elt #(MNode?.h2 tree) path' (MNode?.rnode tree)
+
+
+(*
+ * type for the proof stream which is a list of hashes and looked up data
+ *)
+type proof =
+  | Mk_proof: data:data -> pstream:list hash -> proof
+
+val lenp: proof -> Tot nat
+let lenp p = List.length (Mk_proof?.pstream p)
+
+val p_tail: p:proof{lenp p > 0} -> Tot proof
+let p_tail p = Mk_proof (Mk_proof?.data p) (Cons?.tl (Mk_proof?.pstream p))
+
+let p_data = Mk_proof?.data
+
+let p_stream = Mk_proof?.pstream
+
+(*
+ * verifier takes as input a proof stream for certain lookup path
+ * and computes the expected root node hash
+ *)
+val verifier: path:path -> p:proof{lenp p = List.length path} -> Tot hash
+let rec verifier path p =
+  match path with
+    | [] -> hashFunc (serialize(p_data p))
+
+    | bit::path' ->
+      match p_stream p with
+  | hd::_ ->
+    let h' = verifier path' (p_tail p) in
+    if bit then
+      hashFunc (hashConcat h' hd)
+    else
+      hashFunc (hashConcat hd h')
+
+(*
+ * prover function, generates a proof stream for a path
+ *)
+
+
+val prover: #h:hash ->
+            path:path ->
+            tree:merkleTree (List.length path) h ->
+            Tot (p:proof{lenp p = List.length path})
+      (decreases path)
+
+let rec prover #h path tree =
+  match path with
+    | [] -> Mk_proof (MLeaf?.element tree) []
+    | bit::path' ->
+      let MNode #dc #hl #hr left right  = tree in
+      if bit then
+  let p = prover path' left in
+  Mk_proof (p_data p) (hr::(p_stream p))
+      else
+  let p = prover path' right in
+  Mk_proof (p_data p) (hl::(p_stream p))
+
+(*
+ * correctness theorem: honest prover's proof stream is accepted by the verifier
+ *)
+
+ (*)
+val correctness: #h:hash ->
+                 path:path ->
+                 tree:merkleTree (List.length path) h ->
+                 p:proof{p = prover path tree} ->
+                 Lemma (requires True) (ensures (verifier path p = h))
+                 (decreases path)
+let rec correctness #h path tree p =
+  match path with
+    | [] -> ()
+    | bit::path' ->
+      if bit then
+  correctness #(MNode?.h1 tree) path' (MNode?.lnode tree) (p_tail p)
+      else
+  correctness #(MNode?.h2 tree) path' (MNode?.rnode tree) (p_tail p)
+
+(*
+ * We prove a standard security definition that if verifier can be tricked into
+ * accepting a proof of existence of an element, when the element is not actually
+ * present, then we can provide a constructive proof of hash collision
+ *)
+
+type hash_collision =
+    cexists (fun n -> cexists (fun (s1:data) -> cexists (fun (s2:data) ->
+             u:unit{ s1 = hashFunc s2 /\ not (s1 = s2)})))
+
+(*
+ * security theorem: Only way a verifier can be tricked into accepting proof
+ * stream for an non existent element is if there is a hash collision.
+ *)
+val security: #h:hash ->
+              path:path ->
+              tree:mtree (len path) h ->
+              p:proof{lenp p = len path /\ verifier path p = h /\
+                      not (get_elt path tree = p_data p)} ->
+              Tot hash_collision
+              (decreases path)
+let rec security #h path tree p =
+  match path with
+    | [] -> ExIntro data_size (ExIntro (p_data p) (ExIntro (L?.data tree) ()))
+
+    | bit::path' ->
+      let N #dc #h1 #h2 left right = tree in
+      let h' = verifier path' (p_tail p) in
+      let hd = Cons?.hd (p_stream p) in
+      if bit then
+  if h' = h1 then
+    security path' left (p_tail p)
+  else
+    ExIntro (hash_size + hash_size) (ExIntro (Concat h1 h2) (ExIntro (Concat h' hd) ()))
+      else
+  if h' = h2 then
+    security path' right (p_tail p)
+  else
+    ExIntro (hash_size + hash_size) (ExIntro (Concat h1 h2) (ExIntro (Concat hd h') ()))
+
+*)
+*)
+type claimChain (f: cmpClaim ) = 
+	|InitClaimChain : 
+			nonce: nat ->
+			id: bytes -> (* reference to ClaimChain to have claims that states ClaimChainState and revocation
+			equally it could be used as a ref to chaimChain = skipList + index *) 
 			meta : metadata -> 
-			claims: list claim -> 
-			state: bytes -> 
-			claimChain
+			claims: claimCh f -> 
+			state: bytes -> (* hash? *)
+			hash: bytes {hash = (let c1 = concat (toBytes nonce) id in 
+									let c2 = concat c1 (toBytes meta) in 
+										let c3 = concat c2 (toBytes claims) in 
+											let c4 = concat c3 state in 
+												c4
+								)
+						} -> 
+			claimChain f
 
 
-private val getMetadata: c: claimChain -> metadata
-let getMetadata c = 
-	match c with 
-	| InitChaimChain _ meta _ _ -> meta
+type hash = seq nat
+type data (f: cmpClaim )  = claimChain f
 
-private val getClaims : c: claimChain -> list claim
-let getClaims c = 
-	match c with 
-	| InitChaimChain _ _ claims _ -> claims	
+assume val serialize: #f: cmpClaim ->  d: data f -> Tot(seq nat)
 
-val addElement: c: claimChain -> e: 'a -> Tot ( r: claimChain{getClaims c = getClaims r})
-let addElement c e = 
-	let metadata = getMetadata c in 
-	let blocks = getClaims c in 
-	InitChaimChain c.id metadata blocks c.state
+noeq type merkleTree: level:nat -> h: hash -> Type  = 
+| MLeaf: #f: cmpClaim -> element : data f -> merkleTree 0 (hashFunc (serialize element))
+| MNode: #level: nat -> #h1: hash -> #h2 : hash -> 
+		lnode: merkleTree level h1 ->
+		rnode: merkleTree level h2 -> 
+		merkleTree (level+1) (hashConcat h1 h2)
+
+val mtClChain: f: cmpClaim ->  cl: claimChain f -> merkleTree 0 (hashFunc (serialize cl))
